simple ffi examples
simple ffi examples

- store effect is now more general (can be polymorphic in ctx dep bit)
- delimlang embedded into a language with higher-order heap
- type system + interpretation + safety wrt GITree eq. th.
- an example without glue code, which is well-typed, but
  unguarded shift captures heap lang ctx, which results in a wrong computation

missing build instruction

theories/examples/delim_lang/example.v
@@ -12,46 +12,44 @@ Open Scope syn_scope.
 Example p : expr Empty_set :=
   ((#1) + (reset ((#3) + (shift/cc ((($0) @k #5) + (($0) @k #6)))))).
 
+Global Ltac shift_hom :=
+  match goal with
+  | |- envs_entails _ (wp _ (ofe_mor_car _ _ (λne x, ?k1 x) (?k2 ?t)) _ _ _) =>
+      assert ((ofe_mor_car _ _ (λne x, k1 x) (k2 t)) ≡ (λne x, k1 (k2 x)) t) as -> by done
+  | |- envs_entails _ (wp _ (?k ?t) _ _ _) =>
+      assert (k t ≡ (λne x, k x) t) as -> by done
+  end.
 
-Section example.
-  Local Definition rs : gReifiers _ _ := gReifiers_cons reify_delim gReifiers_nil.
+Global Ltac shift_natop_l :=
+  match goal with
+  | |- envs_entails _ (wp _ (ofe_mor_car _ _ (λne x, ?k1 x)
+                              (ofe_mor_car _ _
+                                 (ofe_mor_car _ _
+                                    (NATOP (do_natop lang.Add)) ?t) (IT_of_V ?e))) _ _ _) =>
+      assert ((ofe_mor_car _ _ (λne x, k1 x) (NATOP (do_natop lang.Add) t (IT_of_V e))) ≡
+                (λne x, k1 (NATOP (do_natop lang.Add) x (IT_of_V e))) t) as -> by done
+  end.
+
+Section proof.
+
+  Context {sz : nat}.
+  Variable rs : gReifiers CtxDep sz.
+  Context `{!subReifier reify_delim rs}.
+
   Notation F := (gReifiers_ops rs).
   Context {R} `{!Cofe R}.
-  Context `{!SubOfe natO R, !SubOfe unitO R}.
+  Context `{!SubOfe natO R}.
   Notation IT := (IT F R).
   Notation ITV := (ITV F R).
-  Context (env : @interp_scope F R _ Empty_set).
 
-  Definition ts := interp_config rs (Cexpr p) env.
-  Definition t := fst ts.
-  Definition σ := snd ts.
-
-
-  Context `{!invGS Σ, !stateG rs R Σ, !heapG rs R Σ}.
+  Context `{!invGS Σ, !stateG rs R Σ}.
   Notation iProp := (iProp Σ).
 
-
-  Ltac shift_hom :=
-    match goal with
-    | |- envs_entails _ (wp _ (ofe_mor_car _ _ (λne x, ?k1 x) (?k2 ?t)) _ _ _) =>
-        assert ((ofe_mor_car _ _ (λne x, k1 x) (k2 t)) ≡ (λne x, k1 (k2 x)) t) as -> by done
-    | |- envs_entails _ (wp _ (?k ?t) _ _ _) =>
-        assert (k t ≡ (λne x, k x) t) as -> by done
-    end.
-
-  Ltac shift_natop_l :=
-    match goal with
-    | |- envs_entails _ (wp _ (ofe_mor_car _ _ (λne x, ?k1 x)
-                                 (ofe_mor_car _ _
-                                    (ofe_mor_car _ _
-                                       (NATOP (do_natop lang.Add)) ?t) (IT_of_V ?e))) _ _ _) =>
-        assert ((ofe_mor_car _ _ (λne x, k1 x) (NATOP (do_natop lang.Add) t (IT_of_V e))) ≡
-                  (λne x, k1 (NATOP (do_natop lang.Add) x (IT_of_V e))) t) as -> by done
-    end.
-
-  Lemma wp_t (s : gitree.weakestpre.stuckness) :
-    has_substate σ -∗
-                      WP@{rs} t @ s {{βv, βv ≡ RetV 18}}.
+  Lemma wp_t σ (s : gitree.weakestpre.stuckness) :
+    (⊢ has_substate σ
+       -∗ WP@{rs} (interp_expr _ p ı_scope) @ s
+            {{ βv, βv ≡ RetV 18
+                   ∗ has_substate σ }})%I.
   Proof.
     Opaque SHIFT APP_CONT.
     iIntros "Hσ".
@@ -106,8 +104,10 @@ Section example.
     iIntros "!> _ Hσ". simpl.
     rewrite IT_of_V_Ret NATOP_Ret.
     simpl. rewrite -(IT_of_V_Ret 18).
-    iApply (wp_pop_end with "Hσ").
-    iIntros "!> _ _".
-    iApply wp_val. done.
+    iApply wp_val.
+    iModIntro.
+    iFrame "Hσ".
+    done.
   Qed.
-End example.
+
+End proof.
