theories/examples/delim_lang/glue.v
@@ -1,0 +1,1244 @@
+From gitrees Require Export prelude gitree lang_generic hom.
+From stdpp Require Import gmap.
+From gitrees.effects Require Import delim store.
+From gitrees.examples.delim_lang Require Import lang interp typing hom.
+From iris.algebra Require Import list gmap.
+From iris.proofmode Require Import base classes tactics environments.
+From iris.base_logic Require Import algebra.
+From iris.heap_lang Require Import locations.
+Require Import Binding.Resolver Binding.Lib Binding.Set Binding.Auto Binding.Env.
+
+From gitrees.examples.delim_lang Require example logpred.
+
+Module embed_lang.
+
+  Definition ty := typing.ty.
+  Definition expr := lang.expr.
+  Definition tyctx {S : Set} := S → ty.
+  Definition typed_expr {S : Set} := typing.typed_expr (S := S).
+  Definition typed_val {S : Set} := typing.typed_val (S := S).
+  Definition interp_closed {sz} (rs : gReifiers CtxDep sz)
+    `{!subReifier reify_delim rs}
+    (e : expr ∅) {R}
+    `{!Cofe R, !SubOfe natO R} : IT (gReifiers_ops rs) R :=
+    interp.interp_expr rs e ı_scope.
+
+End embed_lang.
+
+Section syntax.
+
+  Definition loc : Set := locations.loc.
+  Global Instance loc_dec_eq (l l' : loc) : Decision (l = l') := _.
+
+  Inductive expr {X : Set} :=
+  | Var (x : X) : expr
+  | App (e₁ : expr) (e₂ : expr) : expr
+  | LamV (e : @expr (inc X))
+  | NatOp (op : nat_op) (e₁ : expr) (e₂ : expr) : expr
+  | Alloc (e : expr) : expr
+  | Assign (e₁ e₂ : expr) : expr
+  | Deref (e : expr) : expr
+  | LocV (l : loc)
+  | UnitV
+  | LitV (n : nat)
+  | Embed : embed_lang.expr ∅ → expr.
+
+End syntax.
+
+Arguments expr X%bind : clear implicits.
+
+Section typing.
+
+  Inductive ty :=
+  | tNat
+  | tUnit
+  | tArr (τ1 τ2 : ty)
+  | tRef (τ : ty).
+
+  Inductive typed_glued
+    : forall {S : Set}, (S → ty) → expr S → ty → Type :=
+| typed_GlueNat {S : Set} (Ω : S → ty) α e :
+  embed_lang.typed_expr □ α e α ℕ →
+  typed_glued Ω (Embed e) tNat
+| typed_VarG {S : Set} (Ω : S → ty) (v : S) :
+  typed_glued Ω (Var v) (Ω v)
+| typed_AppG {S : Set} (Ω : S → ty) (τ1 τ2 : ty) e1 e2 :
+  typed_glued Ω e1 (tArr τ1 τ2) →
+  typed_glued Ω e2 τ1 →
+  typed_glued Ω (App e1 e2) τ2
+| typed_AllocG {S : Set} (Ω : S → ty) τ e :
+  typed_glued Ω e τ →
+  typed_glued Ω (Alloc e) (tRef τ)
+| typed_AssignG {S : Set} (Ω : S → ty) (τ : ty) e1 e2 :
+  typed_glued Ω e1 (tRef τ) →
+  typed_glued Ω e2 τ →
+  typed_glued Ω (Assign e1 e2) tUnit
+| typed_DerefG {S : Set} (Ω : S → ty) (τ : ty) e :
+  typed_glued Ω e (tRef τ) →
+  typed_glued Ω (Deref e) τ
+| typed_NatG {S : Set} (Ω : S → ty) n :
+  typed_glued Ω (LitV n) tNat
+| typed_UnitG {S : Set} (Ω : S → ty) :
+  typed_glued Ω UnitV tUnit
+| typed_LamG {S : Set} (Ω : S → ty) (τ1 τ2 : ty) (e : expr (inc S)) :
+  typed_glued (Ω ▹ τ1) e τ2 →
+  typed_glued Ω (LamV e) (tArr τ1 τ2)
+| typed_NatOpG {S : Set} (Ω : S → ty) e1 e2 op :
+  typed_glued Ω e1 tNat →
+  typed_glued Ω e2 tNat →
+  typed_glued Ω (NatOp op e1 e2) tNat.
+
+End typing.
+
+Section interp.
+
+  Context {sz : nat}.
+  Variable rs : gReifiers CtxDep sz.
+  Context `{!subReifier reify_delim rs}.
+  Context `{!subReifier (sReifier_NotCtxDep_min reify_store CtxDep) rs}.
+  Notation F := (gReifiers_ops rs).
+  Context {R} `{!Cofe R}.
+  Context `{!SubOfe natO R}.
+  Context `{!SubOfe unitO R}.
+  Context `{!SubOfe locO R}.
+  Notation IT := (IT F R).
+  Notation ITV := (ITV F R).
+
+  Context `{!invGS Σ, !stateG rs R Σ, !heapG rs R Σ}.
+  Notation iProp := (iProp Σ).
+
+  Definition interp_nat {A} (n : nat) : A -n> IT := λne _,
+      Ret n.
+
+  Definition interp_unit {A} : A -n> IT := λne _, Ret tt.
+
+  Definition interp_loc {A} (l : loc) : A -n> IT := λne _,
+      Ret l.
+
+  Program Definition interp_lam {S : Set} (b : interp_scope (inc S) -n> IT)
+    : interp_scope S -n> IT := λne env, (λit x, (b (extend_scope env x))).
+  Next Obligation.
+    intros; repeat intro; repeat f_equiv; assumption.
+  Qed.
+  Next Obligation.
+    intros; repeat intro; repeat f_equiv; intro; simpl;
+      f_equiv; intro z; simpl.
+    destruct z; done.
+  Qed.
+
+  Program Definition interp_app {A : ofe} (t1 : A -n> IT) (t2 : A -n> IT)
+    : A -n> IT := λne env,
+      LET (t2 env) $ λne x,
+      LET (t1 env) $ λne f,
+      APP' f x.
+  Solve All Obligations with solve_proper_please.
+
+  Program Definition interp_alloc {A} (α : A -n> IT) : A -n> IT := λne env,
+      LET (α env) $ λne α, ALLOC α Ret.
+  Solve All Obligations with solve_proper_please.
+
+  Program Definition interp_deref {A} (α : A -n> IT) : A -n> IT := λne env,
+      flip get_ret (α env) $ λne (l : loc), READ l.
+  Solve All Obligations with solve_proper_please.
+
+  Program Definition interp_assign {A} (α : A -n> IT) (β : A -n> IT) : A -n> IT :=
+    λne env,
+      LET (β env) $ λne β,
+      flip get_ret (α env) $ λne (l : loc),
+      (WRITE l β).
+  Solve All Obligations with solve_proper_please.
+
+  Program Definition interp_natop {A} (op : nat_op) (t1 t2 : A -n> IT) : A -n> IT :=
+    λne env, NATOP (do_natop op) (t1 env) (t2 env).
+  Solve All Obligations with solve_proper_please.
+
+  Program Fixpoint interp_expr {S} (e : expr S) : interp_scope S -n> IT :=
+    match e with
+    | Var x => interp_var x
+    | App n m => interp_app (interp_expr n) (interp_expr m)
+    | LamV e => interp_lam (interp_expr e)
+    | NatOp op n m => interp_natop op (interp_expr n) (interp_expr m)
+    | Alloc e => interp_alloc (interp_expr e)
+    | Assign n m => interp_assign (interp_expr n) (interp_expr m)
+    | Deref e => interp_deref (interp_expr e)
+    | LocV l => interp_loc l
+    | UnitV => interp_unit
+    | LitV n => interp_nat n
+    | Embed e => constO $ (RESET (Next (embed_lang.interp_closed  _ e)))
+    end.
+
+  Section example.
+
+    Definition test_pr1 : expr ∅
+      := App (LamV (Alloc (Var VZ)))
+           (Embed (gitrees.examples.delim_lang.example.p)).
+
+    Lemma p_typ : embed_lang.typed_expr □ ℕ example.p ℕ ℕ.
+    Proof.
+      repeat econstructor.
+    Qed.
+
+    Lemma test_typ1 :
+      typed_glued □ test_pr1 (tRef tNat).
+    Proof.
+      repeat econstructor.
+      constructor. (* ??? wtf ??? *)
+    Qed.
+
+    Lemma test_helper_prop1 :
+      ⊢ ∀ x σ (Φ : ITV → iProp), has_substate (laterO_map x :: σ : delim.stateF ♯ IT)
+        -∗ (∀ v, v ≡ RetV 18 -∗ has_substate (σ : delim.stateF ♯ IT) -∗ WP@{rs} (x (IT_of_V v)) {{ Φ }})
+        -∗ WP@{rs} 𝒫 (delim_lang.interp.interp_expr rs example.p ı_scope) {{ Φ }}.
+    Proof.
+      Opaque SHIFT APP_CONT.
+      iIntros (x σ Φ) "Hσ HΦ".
+      cbn.
+      do 2 example.shift_hom.
+      iApply (wp_reset with "Hσ").
+      iIntros "!> _ Hσ". simpl.
+
+      do 2 example.shift_hom.
+      iApply (wp_shift with "Hσ").
+      { rewrite laterO_map_Next. done. }
+      iIntros "!>_ Hσ".
+      simpl.
+
+      (* the rest *)
+      rewrite -(IT_of_V_Ret 6) get_val_ITV'. simpl.
+      rewrite get_fun_fun. simpl.
+      do 2 example.shift_hom.
+      iApply (wp_app_cont with "Hσ"); first done.
+      iIntros "!> _ Hσ". simpl.
+      rewrite later_map_Next -Tick_eq.
+      iApply wp_tick. iNext.
+      example.shift_hom.
+      rewrite IT_of_V_Ret NATOP_Ret. simpl.
+      rewrite -(IT_of_V_Ret 9).
+      iApply (wp_pop_cons with "Hσ").
+      iIntros "!> _ Hσ".
+      simpl.
+
+      example.shift_hom. example.shift_natop_l.
+      rewrite -(IT_of_V_Ret 5) get_val_ITV'. simpl.
+      example.shift_hom. example.shift_natop_l.
+      rewrite get_fun_fun. simpl.
+      example.shift_hom. example.shift_natop_l.
+      iApply (wp_app_cont with "Hσ"); first done.
+      iIntros "!> _ Hσ". simpl.
+      rewrite later_map_Next -Tick_eq.
+      iApply wp_tick. iNext.
+      rewrite (IT_of_V_Ret 5) NATOP_Ret. simpl.
+      rewrite -(IT_of_V_Ret 8).
+      iApply (wp_pop_cons with "Hσ").
+      iIntros "!> _ Hσ".
+      simpl.
+      example.shift_hom.
+      example.shift_natop_l.
+      rewrite (IT_of_V_Ret 8).
+      simpl. rewrite IT_of_V_Ret NATOP_Ret.
+      simpl. rewrite -(IT_of_V_Ret 17).
+      iApply (wp_pop_cons with "Hσ").
+      iIntros "!> _ Hσ". simpl.
+      rewrite IT_of_V_Ret NATOP_Ret.
+      simpl. rewrite -(IT_of_V_Ret 18).
+
+      iApply (wp_pop_cons with "Hσ").
+      iIntros "!> _ Hσ".
+      by iApply "HΦ".
+    Qed.
+
+    Lemma test_prop1 σ :
+      ⊢ heap_ctx rs
+        -∗ has_substate (σ : delim.stateF ♯ IT)
+        -∗ WP@{rs} (interp_expr test_pr1 ı_scope) @ notStuck
+             {{ βv, ∃ (l : loc),
+                      βv ≡ RetV l
+                      ∗ pointsto l (Ret 18)
+                      ∗ has_substate (σ : delim.stateF ♯ IT)}}.
+    Proof.
+      Opaque SHIFT APP_CONT RESET gitrees.examples.delim_lang.example.p.
+      iIntros "T H".
+      cbn.
+
+      match goal with
+      | |- context G [ofe_mor_car _ _ (ofe_mor_car _ _ LET ?a) ?b] =>
+          set (F := b)
+      end.
+      unshelve eset (K := (exist _ (LETCTX F) _ : HOM)).
+      { apply _. }
+
+      iApply (wp_reset with "H").
+      iNext.
+      iIntros "? H".
+      iApply (test_helper_prop1 $! (get_val F) σ with "H").
+      iIntros (v) "#HEQ H".
+      subst F.
+      simpl.
+      rewrite get_val_ITV.
+      simpl.
+      rewrite LET_Val.
+      simpl.
+      rewrite APP'_Fun_l.
+      simpl.
+      rewrite <-Tick_eq.
+      iApply wp_tick.
+      iNext.
+      rewrite LET_Val.
+      simpl.
+      iApply (wp_alloc with "T").
+      { solve_proper. }
+      do 2 iNext.
+      iIntros (l) "Hl".
+      iApply wp_val.
+      iModIntro.
+      iExists l.
+      iSplit; first done.
+      iFrame "H".
+      assert (Ret 18 ≡ IT_of_V (RetV 18))%stdpp as ->.
+      { by rewrite -(IT_of_V_Ret 18). }
+      iRewrite - "HEQ".
+      done.
+    Qed.
+
+    Definition test_pr2' : embed_lang.expr ∅
+      := (rec (reset (reset (if ($ 0) then (# 1) else (# 0)))))%syn.
+
+    (* glue rule for functions might be a problem,
+       since it should relate src level functions of type τ → σ to
+      ∀ α. τ' ∕ α → σ' ∕ α, where τ, σ are pairwise compatible with τ', σ' *)
+    Lemma test_typ2' α β : embed_lang.typed_expr □ β test_pr2' (ℕ ∕ α → ℕ ∕ α) β.
+    Proof.
+      repeat econstructor.
+    Qed.
+
+    Definition test_pr2 : expr ∅
+      := App (Embed test_pr2') (LitV 0).
+
+    Lemma test_prop2 σ :
+      ⊢ heap_ctx rs
+        -∗ has_substate (σ : delim.stateF ♯ IT)
+        -∗ WP@{rs} (interp_expr test_pr2 ı_scope) @ notStuck
+             {{ βv, βv ≡ RetV 0
+                      ∗ has_substate (σ : delim.stateF ♯ IT)}}.
+    Proof.
+      Opaque test_pr2'.
+      iIntros "T H".
+      cbn.
+      rewrite LET_Val.
+      simpl.
+
+      match goal with
+      | |- context G [ofe_mor_car _ _ (ofe_mor_car _ _ LET ?a) ?b] =>
+          set (F := b)
+      end.
+      unshelve eset (K := (exist _ (LETCTX F) _ : HOM)).
+      { apply _. }
+
+      iApply (wp_reset with "H").
+      iNext.
+      iIntros "? H".
+      Transparent test_pr2'.
+      simpl.
+      unfold embed_lang.interp_closed.
+      unfold test_pr2'.
+      simpl.
+      unfold delim_lang.interp.interp_expr.
+      simpl.
+      rewrite interp_rec_unfold.
+      iApply (wp_pop_cons with "H").
+      iIntros "!> _ Hσ".
+      rewrite get_val_fun.
+      subst K F.
+      simpl.
+      rewrite APP'_Fun_l.
+      simpl.
+      rewrite -Tick_eq.
+      iApply wp_tick.
+      iNext.
+      rewrite IF_False; last lia.
+      match goal with
+      | |- context G [ofe_mor_car _ _ RESET ?a] =>
+          assert (ofe_mor_car _ _ RESET a = idfun $ ofe_mor_car _ _ RESET a) as ->
+      end; first reflexivity.
+      iApply (wp_reset with "Hσ").
+      iIntros "!> _ Hσ".
+      rewrite get_val_vis.
+      iApply (wp_subreify_ctx_dep _ _ _ _ _ _ _ (Next $ 𝒫 (Ret 0)) with "Hσ").
+      { simpl. rewrite later_map_Next. reflexivity. }
+      { reflexivity. }
+      iIntros "!> _ Hσ".
+      match goal with
+      | |- context G [?f :: _] =>
+          assert (f ≡ laterO_map 𝒫)%stdpp as ->
+      end.
+      {
+        intro; simpl.
+        rewrite ofe_iso_21.
+        reflexivity.
+      }
+      iApply (wp_pop_cons with "Hσ").
+      iIntros "!> _ Hσ".
+      iApply (wp_pop_cons with "Hσ").
+      iIntros "!> _ Hσ".
+      iApply wp_val.
+      iModIntro.
+      by iSplit.
+    Qed.
+  End example.
+End interp.
+
+Section sets.
+
+  Context {sz : nat}.
+  Variable rs : gReifiers CtxDep sz.
+  Context `{!subReifier reify_delim rs}.
+  Context `{!subReifier (sReifier_NotCtxDep_min reify_store CtxDep) rs}.
+  Notation F := (gReifiers_ops rs).
+  Context {R} {CR : Cofe R}.
+  Context `{!SubOfe natO R}.
+  Context `{!SubOfe unitO R}.
+  Context `{!SubOfe locO R}.
+  Notation IT := (IT F R).
+  Notation ITV := (ITV F R).
+
+  Context `{!invGS Σ, !stateG rs R Σ, !heapG rs R Σ}.
+  Notation iProp := (iProp Σ).
+
+  Canonical Structure exprO S := leibnizO (expr S).
+
+  Notation "'WP' α {{ β , Φ } }" := (wp rs α notStuck ⊤ (λ β, Φ))
+    (at level 20, α, Φ at level 200,
+     format "'WP'  α  {{  β ,  Φ  } }") : bi_scope.
+  Notation "'WP' α {{ Φ } }" := (wp rs α notStuck ⊤ Φ)
+    (at level 20, α, Φ at level 200,
+     format "'WP'  α  {{  Φ  } }") : bi_scope.
+
+  Program Definition interp_tnat : ITV -n> iProp := λne αv,
+      (∃ n : nat, αv ≡ RetV n)%I.
+  Solve All Obligations with solve_proper_please.
+
+  Program Definition interp_tunit : ITV -n> iProp := λne αv,
+      (αv ≡ RetV ())%I.
+  Solve All Obligations with solve_proper_please.
+
+  Program Definition obs_ref : IT -n> iProp :=
+    λne α,
+      (has_substate ([] : delim.stateF ♯ IT)
+       -∗ WP (𝒫 α) {{ βv, has_substate ([] : delim.stateF ♯ IT) }})%I.
+  Next Obligation. solve_proper_please. Qed.
+
+  Definition logrel_ectx V (κ : HOM) : iProp :=
+    (□ ∀ (βv : ITV), V βv -∗ obs_ref (`κ (IT_of_V βv)))%I.
+
+  Program Definition interp_tarr (Φ1 Φ2 : ITV -n> iProp)
+    : ITV -n> iProp :=
+    λne αv,
+      (∃ f', IT_of_V αv ≡ Fun f'
+             ∧ □ ∀ βv, Φ1 βv -∗ ∀ (κ : HOM), logrel_ectx Φ2 κ -∗ obs_ref (`κ ((Fun f') ⊙ ((IT_of_V βv)))))%I.
+  Solve All Obligations with solve_proper_please.
+
+  Definition logN : namespace := nroot .@ "logN".
+
+  Program Definition interp_ref (Φ : ITV -n> iProp) : ITV -n> iProp := λne αv,
+      (∃ (l : loc), αv ≡ RetV l ∗ inv (logN .@ l) (∃ βv, pointsto l (IT_of_V βv) ∗ Φ βv))%I.
+  Solve All Obligations with solve_proper_please.
+
+  Fixpoint interp_ty (τ : ty) : ITV -n> iProp :=
+    match τ with
+    | tUnit => interp_tunit
+    | tNat  => interp_tnat
+    | tArr τ1 τ2 => interp_tarr (interp_ty τ1) (interp_ty τ2)
+    | tRef τ => interp_ref (interp_ty τ)
+    end.
+
+  Global Instance interp_ty_persistent (τ : ty) α :
+    Persistent (interp_ty τ α).
+  Proof.
+    revert α. induction τ=> α; simpl.
+    - apply _.
+    - apply _.
+    - apply _.
+    - apply _.
+  Qed.
+
+  Program Definition interp_exprG V : IT -n> iProp :=
+    λne e, (∀ κ, heap_ctx rs
+                 -∗ logrel_ectx V κ
+                 -∗ obs_ref (`κ e))%I.
+  Solve All Obligations with solve_proper_please.
+
+  Program Definition ssubst_validG {S : Set}
+    (Γ : S -> ty)
+    (ss : interp_scope S) : iProp :=
+    (∀ x, □ interp_exprG (interp_ty (Γ x)) (ss x))%I.
+
+  Program Definition validG {S : Set}
+    (Γ : S -> ty)
+    (α : interp_scope S -n> IT)
+    (τ : ty) : iProp :=
+    (□ ∀ (ss : interp_scope S),
+       ssubst_validG Γ ss → interp_exprG (interp_ty τ) (α ss))%I.
+
+  Lemma compat_nat {S : Set} n (Ω : S → ty) :
+    ⊢ validG Ω (interp_nat rs n) tNat.
+  Proof.
+    iModIntro.
+    iIntros (γ) "#H".
+    iIntros (κ) "#Q #W".
+    iIntros "R".
+    iSpecialize ("W" $! (RetV n) with "[] [$R]").
+    - by iExists _.
+    - by iApply "W".
+  Qed.
+
+  Lemma compat_unit {S : Set} (Ω : S → ty) :
+    ⊢ validG Ω (interp_unit rs) tUnit.
+  Proof.
+    iModIntro.
+    iIntros (γ) "#H".
+    iIntros (κ) "#Q #W".
+    iIntros "R".
+    iSpecialize ("W" $! (RetV ()) with "[] [$R]"); first done.
+    by iApply "W".
+  Qed.
+
+  Lemma compat_var {S : Set} (Ω : S → ty) (v : S) :
+    ⊢ validG Ω (interp_var v) (Ω v).
+  Proof.
+    iModIntro.
+    iIntros (γ) "#H".
+    iIntros (κ) "Q W".
+    iIntros "R".
+    iApply ("H" with "Q W R").
+  Qed.
+
+  Lemma compat_app {S : Set}
+    (Ω : S → ty)
+    α β τ1 τ2 :
+    ⊢ validG Ω α (tArr τ1 τ2)
+      -∗ validG Ω β τ1
+      -∗ validG Ω (interp_app _ α β) τ2.
+  Proof.
+    iIntros "#H #G".
+    iModIntro.
+    iIntros (γ) "#Hγ".
+    iIntros (κ) "#Q #W".
+    iIntros "R".
+    simpl.
+    match goal with
+    | |- context G [ofe_mor_car _ _ (ofe_mor_car _ _ LET ?a) ?b] =>
+        set (F := b)
+    end.
+    unshelve eset (K := (exist _ (LETCTX F) _ : HOM)).
+    { apply _. }
+    assert ((LET (β γ) F) ≡ `K (β γ))%stdpp as ->.
+    { reflexivity. }
+    rewrite HOM_ccompose.
+    iSpecialize ("G" $! γ with "Hγ").
+    iSpecialize ("G" $! (HOM_compose κ K)).
+    iApply ("G" with "Q [] R").
+    iClear "G".
+    iIntros (v).
+    iModIntro.
+    iIntros "#Hv".
+    iIntros "R".
+    simpl.
+    rewrite LET_Val.
+    subst F K.
+    simpl.
+    match goal with
+    | |- context G [ofe_mor_car _ _ (ofe_mor_car _ _ LET ?a) ?b] =>
+        set (F := b)
+    end.
+    unshelve eset (K := (exist _ (LETCTX F) _ : HOM)).
+    { apply _. }
+    assert ((LET (α γ) F) ≡ `K (α γ))%stdpp as ->.
+    { reflexivity. }
+    rewrite HOM_ccompose.
+    iSpecialize ("H" $! γ with "Hγ").
+    iSpecialize ("H" $! (HOM_compose κ K)).
+    iApply ("H" with "Q [] R").
+    iIntros (w).
+    iModIntro.
+    iIntros "#Hw".
+    iIntros "R".
+    simpl.
+    rewrite LET_Val.
+    subst F.
+    simpl.
+    iDestruct "Hw" as "(%f & #HEQ & #Hw)".
+    iAssert ((IT_of_V w ⊙ (IT_of_V v)) ≡ (Fun f ⊙ (IT_of_V v)))%I as "HEQ'".
+    {
+      iApply (f_equivI (flipO APP' (IT_of_V v))).
+      iApply "HEQ".
+    }
+    iRewrite "HEQ'".
+    iApply ("Hw" with "Hv [] R").
+    iApply "W".
+  Qed.
+
+  Lemma compat_alloc {S : Set}
+    (Ω : S → ty)
+    (τ : ty)
+    (e : expr S) :
+    ⊢ validG Ω (interp_expr rs e) τ -∗ validG Ω (interp_expr rs (Alloc e)) (tRef τ).
+  Proof.
+    iIntros "#H".
+    iModIntro.
+    iIntros (γ) "#Hγ".
+    iIntros (κ) "#Q #W".
+    iIntros "R".
+    simpl.
+    match goal with
+    | |- context G [ofe_mor_car _ _ (ofe_mor_car _ _ LET ?a) ?b] =>
+        set (F := b)
+    end.
+    unshelve eset (K := HOM_compose κ (exist _ (LETCTX F) _ : HOM)).
+    { apply _. }
+    iSpecialize ("H" $! γ with "Hγ").
+    iSpecialize ("H" $! K with "Q [] R"); first last.
+    { subst K; simpl; iApply "H". }
+    iIntros (v).
+    iModIntro.
+    iIntros "#Hv".
+    iIntros "T".
+    subst K.
+    simpl.
+    rewrite LET_Val.
+    subst F.
+    cbn [ofe_mor_car].
+    do 2 rewrite hom_vis.
+    iApply wp_subreify_ctx_indep_lift''. simpl.
+    iInv (nroot.@"storeE") as (σ) "[>Hlc [Hs Hh]]" "Hcl".
+    iApply (lc_fupd_elim_later with "Hlc").
+    iModIntro.
+    set (l:=Loc.fresh (dom σ)).
+    iExists σ, l, _, (𝒫 (`κ (Ret l))).
+    iFrame "Hs".
+    simpl. change (Loc.fresh (dom σ)) with l.
+    iSplit; first done.
+    iSplit.
+    { simpl. rewrite ofe_iso_21. done. }
+    iNext. iIntros "Hlc Hs".
+    iMod (istate_alloc _ (IT_of_V v) l with "Hh") as "[Hh Hl]".
+    {
+      apply (not_elem_of_dom_1 (M:=gmap loc)).
+      rewrite -(Loc.add_0 l). apply Loc.fresh_fresh. lia.
+    }
+    iMod (inv_alloc (logN.@l) _
+            (∃ βv : ITV, pointsto l (IT_of_V βv) ∗ interp_ty τ βv) with "[Hl Hv]")
+      as "#HN".
+    {
+      iNext.
+      iExists v.
+      iFrame.
+      iFrame "Hv".
+    }
+    iMod ("Hcl" with "[Hlc Hh Hs]") as "_".
+    { iExists _. by iFrame. }
+    iSpecialize ("W" $! (RetV l) with "[]").
+    {
+      iExists l.
+      iSplit; first done.
+      iApply "HN".
+    }
+    iSpecialize ("W" with "T").
+    iModIntro.
+    iApply "W".
+  Qed.
+
+  Lemma compat_assign {S : Set} {Ω : S → ty}
+    τ e1 e2
+    : validG Ω (interp_expr rs e1) (tRef τ)
+      -∗ validG Ω (interp_expr rs e2) τ
+      -∗ validG Ω (interp_expr rs (Assign e1 e2)) tUnit.
+  Proof.
+    iIntros "#H #G".
+    iModIntro.
+    iIntros (γ) "#Hγ".
+    iIntros (κ) "#Hheap #Hκ".
+    iIntros "Hst".
+    simpl.
+    match goal with
+    | |- context G [ofe_mor_car _ _ (ofe_mor_car _ _ LET ?a) ?b] =>
+        set (F := b)
+    end.
+    unshelve eset (K := HOM_compose κ (exist _ (LETCTX F) _ : HOM)).
+    { apply _. }
+    iSpecialize ("G" $! γ with "Hγ").
+    iSpecialize ("G" $! K with "Hheap [] Hst"); first last.
+    { subst K; simpl; iApply "G". }
+    iIntros (v).
+    iModIntro.
+    iIntros "#Hv".
+    iIntros "Hst".
+    subst K.
+    simpl.
+    rewrite LET_Val.
+    subst F.
+    simpl.
+    match goal with
+    | |- context G [get_ret ?a] =>
+          set (F := a)
+    end.
+    unshelve eset (K := HOM_compose κ (exist _ (get_ret F) _) : HOM).
+    { apply _. }
+    iSpecialize ("H" $! γ with "Hγ").
+    iSpecialize ("H" $! K with "Hheap [] Hst"); first last.
+    { subst K; simpl; iApply "H". }
+    iIntros (w).
+    iModIntro.
+    subst K F.
+    simpl.
+    iIntros "(%l & #HEQ & Hw)".
+    iIntros "Hst".
+    iRewrite "HEQ".
+    rewrite IT_of_V_Ret.
+    rewrite get_ret_ret.
+    simpl.
+    do 2 rewrite hom_vis.
+
+    iApply wp_subreify_ctx_indep_lift''. simpl.
+    iInv (nroot.@"storeE") as (σ) "[>Hlc [Hs Hh]]" "Hcl".
+    iApply (fupd_mask_weaken (⊤ ∖ nclose (nroot.@"storeE"))).
+    { set_solver. }
+    iIntros "Hwk".
+    iInv (logN.@l) as "H" "Hcl'".
+    iAssert (▷ ⌜is_Some (σ !! l)⌝)%I as "#Hdom".
+    {
+      iNext.
+      iDestruct "H" as "(%βv & Hp & H)".
+      iApply (istate_loc_dom with "Hh Hp").
+    }
+    iDestruct "Hdom" as ">%Hdom".
+    destruct Hdom as [x Hx].
+    destruct (Next_uninj x) as [α' Ha'].
+    iApply (lc_fupd_elim_later with "Hlc").
+    iNext.
+    iExists σ, (), (<[l:=Next (IT_of_V v)]>σ), (𝒫 (`κ (Ret ()))).
+    iFrame "Hs".
+    iSimpl. repeat iSplit; [done | done | ].
+    iNext. iIntros "Hlc".
+    iDestruct "H" as "(%βv & Hp & H)".
+    iMod (istate_write _ _ (IT_of_V βv) (IT_of_V v) with "Hh Hp") as "[Hh Hp]".
+    iIntros "Hs".
+    iMod ("Hcl'" with "[Hp]") as "_".
+    {
+      iNext.
+      iExists v.
+      iFrame.
+      iFrame "Hv".
+    }
+    iMod ("Hcl" with "[Hlc Hh Hs]") as "_".
+    { iExists _. by iFrame. }
+    iModIntro.
+    rewrite <-IT_of_V_Ret.
+    by iApply ("Hκ" with "[] Hst").
+  Qed.
+
+  Lemma compat_deref {S : Set} (Ω : S → ty)
+    τ e
+    : validG Ω (interp_expr rs e) (tRef τ)
+      -∗ validG Ω (interp_expr rs (Deref e)) τ.
+  Proof.
+    iIntros "#H".
+    iModIntro.
+    iIntros (γ) "#Hγ".
+    iIntros (κ) "#Hheap #Hκ".
+    iIntros "Hst".
+    simpl.
+    match goal with
+    | |- context G [get_ret ?a] =>
+          set (F := a)
+    end.
+    unshelve eset (K := HOM_compose κ (exist _ (get_ret F) _) : HOM).
+    { apply _. }
+    iSpecialize ("H" $! γ with "Hγ").
+    iSpecialize ("H" $! K with "Hheap [] Hst"); first last.
+    { subst K; simpl; iApply "H". }
+    iIntros (w).
+    iModIntro.
+    iIntros "#Hw".
+    iIntros "Hst".
+    subst K F.
+    simpl.
+    iDestruct "Hw" as "(%l & #HEQ & Hw)".
+    iRewrite "HEQ".
+    rewrite IT_of_V_Ret.
+    rewrite get_ret_ret.
+    simpl.
+    do 2 rewrite hom_vis.
+
+    iApply wp_subreify_ctx_indep_lift''. simpl.
+    iInv (nroot.@"storeE") as (σ) "[>Hlc [Hs Hh]]" "Hcl".
+    iApply (fupd_mask_weaken (⊤ ∖ nclose (nroot.@"storeE"))).
+    { set_solver. }
+    iIntros "Hwk".
+    iInv (logN.@l) as "H" "Hcl'".
+    iApply (lc_fupd_elim_later with "Hlc").
+    iNext.
+    iDestruct "H" as "(%βv & Hp & #H)".
+    iAssert (⌜is_Some (σ !! l)⌝)%I as "%Hdom".
+    { iApply (istate_loc_dom with "Hh Hp"). }
+    destruct Hdom as [x Hx].
+    destruct (Next_uninj x) as [β' Hb'].
+    iAssert ((σ !! l ≡ Some (Next (IT_of_V βv))))%I as "#Hlookup".
+    { iApply (istate_read with "Hh Hp"). }
+    iAssert (▷ (β' ≡ IT_of_V βv))%I as "#Hba".
+    { rewrite Hx. rewrite option_equivI.
+      rewrite Hb'. by iNext. }
+    iClear "Hlookup".
+    iExists σ, (Next β'), σ, (𝒫 (`κ β')).
+    iFrame "Hs".
+    iSimpl. repeat iSplit; [ | | ].
+    { by rewrite Hx /= Hb'. }
+    {
+      iPureIntro.
+      rewrite ofe_iso_21.
+      reflexivity.
+    }
+    iNext. iIntros "Hlc".
+    iIntros "Hσ".
+    iMod ("Hcl'" with "[Hp H]") as "_".
+    {
+      iNext.
+      iExists βv.
+      iFrame.
+      iFrame "H".
+    }
+    iMod ("Hcl" with "[Hlc Hh Hσ]") as "_".
+    { iNext. iExists _. iFrame. }
+    iModIntro.
+    iRewrite "Hba".
+    iApply ("Hκ" with "H Hst").
+  Qed.
+
+  Lemma compat_natop {S : Set}
+    (Ω : S → ty)
+    op α β :
+    ⊢ validG Ω α tNat
+      -∗ validG Ω β tNat
+      -∗ validG Ω (interp_natop _ op α β) tNat.
+  Proof.
+    iIntros "#H #G".
+    iModIntro.
+    iIntros (γ) "#Hγ".
+    iIntros (κ) "#Q #W".
+    iIntros "R".
+    simpl.
+
+    set (K' := (NatOpRSCtx_HOM op α γ)).
+    assert ((NATOP (do_natop op) (α γ) (β γ)) = ((`K') (β γ))) as -> by done.
+    rewrite HOM_ccompose.
+    pose (sss := (HOM_compose κ K')). rewrite (HOM_compose_ccompose κ K' sss)//.
+
+    iSpecialize ("G" $! γ with "Hγ").
+    iSpecialize ("G" $! sss).
+    iApply ("G" with "Q [] R").
+    iClear "G".
+    iIntros (v).
+    iModIntro.
+    iIntros "#Hv".
+    iIntros "R".
+    simpl.
+    clear K' sss.
+
+    pose (K' := (NatOpLSCtx_HOM op (IT_of_V v) γ _)).
+    assert ((NATOP (do_natop op) (α γ) (IT_of_V v)) = ((`K') (α γ)))
+      as -> by done.
+    rewrite HOM_ccompose.
+    pose (sss := (HOM_compose κ K')). rewrite (HOM_compose_ccompose κ K' sss)//.
+
+    iSpecialize ("H" $! γ with "Hγ").
+    iSpecialize ("H" $! sss).
+    iApply ("H" with "Q [] R").
+    iIntros (w).
+    iModIntro.
+    iIntros "#Hw".
+    iIntros "R".
+    simpl.
+
+    iDestruct "Hv" as "(%n & #HEQ)".
+    iDestruct "Hw" as "(%n' & #HEQ')".
+    iAssert ((NATOP (do_natop op) (IT_of_V w) (IT_of_V v))
+               ≡ (Ret (do_natop op n' n)))%I as "#HEQ''".
+    {
+      iRewrite "HEQ".
+      rewrite IT_of_V_Ret.
+      iAssert ((IT_of_V w) ≡ IT_of_V (RetV n'))%I as "#HEQ2''".
+      {
+        iApply f_equivI.
+        iApply "HEQ'".
+      }
+      rewrite IT_of_V_Ret.
+      iAssert (NATOP (do_natop op) (IT_of_V w) (Ret n)
+                 ≡ NATOP (do_natop op) (Ret n') (Ret n))%I as "#HEQ2'''".
+      {
+        unshelve iApply (f_equivI (λne x, NATOP (do_natop op) x (Ret n))).
+        { solve_proper. }
+        { solve_proper. }
+        iApply "HEQ2''".
+      }
+      iRewrite "HEQ2'''".
+      rewrite NATOP_Ret.
+      done.
+    }
+    iRewrite "HEQ''".
+    rewrite <-IT_of_V_Ret.
+    iApply "W".
+    - by iExists _.
+    - iFrame "R".
+  Qed.
+
+  Lemma compat_lam {S : Set} (Ω : S → ty)
+    (e : expr (inc S))
+    (τ1 τ2 : ty)
+    : ⊢ validG (Ω ▹ τ1) (interp_expr rs e) τ2 -∗ validG Ω (interp_expr rs (LamV e)) (tArr τ1 τ2).
+  Proof.
+    iIntros "#H".
+    iModIntro.
+    iIntros (γ) "#Hγ".
+    iIntros (κ) "#Q #W".
+    iIntros "R".
+    cbn [interp_expr].
+    unfold interp_lam.
+    cbn [ofe_mor_car].
+    match goal with
+    | |- context G [ofe_mor_car _ _ Fun ?a] =>
+        set (F := a)
+    end.
+    assert (Fun F ≡ IT_of_V $ FunV F)%stdpp as ->.
+    { reflexivity. }
+    iApply "W"; last iApply "R".
+    iExists _.
+    iSplit; first done.
+    iModIntro.
+    iIntros (v) "#Hv".
+    fold (interp_ty τ1).
+    fold (interp_ty τ2).
+    iIntros (κ') "#Hκ'".
+    iIntros "Hm'".
+    rewrite APP'_Fun_l.
+    rewrite laterO_map_Next.
+    rewrite <-Tick_eq.
+    iSpecialize ("H" $! (extend_scope γ (IT_of_V v)) with "[]").
+    {
+      iIntros ([| x]); iModIntro.
+      - iIntros (κ'') "? Hκ''".
+        iIntros "?".
+        iApply "Hκ''"; first iApply "Hv".
+        iFrame.
+      - iIntros (κ'') "? #Hκ''".
+        iIntros "?".
+        iApply "Hγ";
+          [iFrame "Q" | iApply "Hκ''" | iFrame].
+    }
+    iSpecialize ("H" $! κ' with "Q [Hκ']"); first iApply "Hκ'".
+    rewrite ->2 hom_tick.
+    iApply wp_tick.
+    iNext.
+    iApply ("H" with "Hm'").
+  Qed.
+
+  Lemma compat_glueNat {S : Set} (Ω : S → ty)
+    (τ : embed_lang.ty)
+    (e : lang.expr ∅)
+    (t : embed_lang.typed_expr □ τ e τ ℕ)
+    : ⊢ validG Ω (interp_expr rs (Embed e)) tNat.
+  Proof.
+    iModIntro.
+    iIntros (γ) "#H".
+    iIntros (κ) "#Q #W".
+    iIntros "R".
+
+    unshelve eset (F := (exist _ (𝒫 : IT -n> IT) _ : HOM)).
+    { apply _. }
+    assert (𝒫 = `F)%stdpp as ->.
+    { done. }
+    rewrite HOM_ccompose.
+    iApply (wp_reset with "R").
+    iNext.
+    iIntros "? R".
+
+    iPoseProof (logpred.fundamental_expr rs □ τ τ ℕ e t) as "#G".
+    unshelve iSpecialize ("G" $! ı_scope _).
+    { iIntros ([]). }
+    iSpecialize ("G" $! HOM_id with "[]").
+    {
+      iIntros (v).
+      iModIntro.
+      iIntros "Hv".
+      iIntros (σ) "Hσ".
+      iIntros "R".
+      iApply ("Hσ" $! v with "Hv R").
+    }
+    iSpecialize ("G" $! (laterO_map (`F ◎ `κ) :: []) with "[W]").
+    {
+      iIntros (?) "K L".
+      iApply (wp_pop_cons with "L").
+      iNext.
+      iIntros "? ?".
+      subst F.
+      simpl.
+      iApply ("W" $! αv with "[K]").
+      - iApply "K".
+      - iFrame.
+    }
+    by iApply "G".
+  Qed.
+
+  Fixpoint fl {S : Set} (Ω : S → ty) (e : expr S) (τ : ty) (H : typed_glued Ω e τ)
+    : ⊢ validG Ω (interp_expr _ e) τ.
+  Proof.
+    destruct H.
+    - by iApply compat_glueNat.
+    - iApply compat_var.
+    - iApply compat_app;
+        [by iApply fl | by iApply fl].
+    - iApply compat_alloc; by iApply fl.
+    - iApply compat_assign;
+        [by iApply fl | by iApply fl].
+    - iApply compat_deref; by iApply fl.
+    - iApply compat_nat.
+    - iApply compat_unit.
+    - iApply compat_lam; by iApply fl.
+    - iApply compat_natop;
+        [by iApply fl | by iApply fl].
+  Qed.
+
+  Lemma compat_HOM_id P :
+    ⊢ logrel_ectx P HOM_id.
+  Proof.
+    iIntros (v).
+    iModIntro.
+    iIntros "Pv Hσ".
+    iApply (wp_pop_end with "Hσ").
+    iIntros "!> _ Hσ".
+    by iApply wp_val.
+  Qed.
+
+End sets.
+
+Local Definition rs : gReifiers CtxDep 2 :=
+  gReifiers_cons reify_delim (gReifiers_cons (sReifier_NotCtxDep_min reify_store CtxDep) gReifiers_nil).
+
+Variable Hdisj : ∀ (Σ : gFunctors) (P Q : iProp Σ), disjunction_property P Q.
+
+Lemma logpred_adequacy cr Σ R `{!Cofe R, SubOfe natO R, SubOfe unitO R, SubOfe locO R}
+  `{!invGpreS Σ} `{!heapPreG rs R Σ} `{!statePreG rs R Σ} τ
+  (α : interp_scope ∅ -n> IT (gReifiers_ops rs) R)
+  (e : IT (gReifiers_ops rs) R) st' k :
+  (∀ `{H1 : !invGS Σ} `{H2: !stateG rs R Σ} `{H3: !heapG rs R Σ},
+      (£ cr ⊢ validG rs □ α τ)%I) →
+  ssteps (gReifiers_sReifier rs) (𝒫 (α ı_scope)) ([], (empty, ())) e st' k →
+  (∃ β1 st1, sstep (gReifiers_sReifier rs) e st' β1 st1)
+   ∨ (∃ βv, (IT_of_V βv ≡ e)%stdpp).
+Proof.
+  intros Hlog Hst.
+  destruct (IT_to_V e) as [βv|] eqn:Hb.
+  { right. exists βv. apply IT_of_to_V'. rewrite Hb; eauto. }
+  left.
+  cut ((∃ β1 st1, sstep (gReifiers_sReifier rs) e st' β1 st1)
+      ∨ (∃ e', (e ≡ Err e')%stdpp ∧ notStuck e')).
+  { intros [?|He]; first done.
+    destruct He as [? [? []]]. }
+  eapply (wp_safety (S cr)); eauto.
+  { apply Hdisj. }
+  { by rewrite Hb. }
+  intros H2 H3.
+  exists (λ _, True)%I. split.
+  { apply _. }
+  iIntros "[[Hone Hcr] Hst]".
+  match goal with
+  | |- context G [has_full_state ?a] =>
+      set (st := a)
+  end.
+  pose (cont_stack := st.1).
+  pose (heap := st.2.1).
+  iMod (new_heapG rs heap) as (H4) "H".
+  iAssert (has_substate (cont_stack : delim.stateF ♯ _) ∗ has_substate heap)%I with "[Hst]" as "[Hcont Hheap]".
+  { unfold has_substate, has_full_state.
+    assert (of_state rs (IT (gReifiers_ops rs) _) st ≡
+            of_idx rs (IT (gReifiers_ops rs) _) sR_idx (sR_state (cont_stack : delim.stateF ♯ _))
+            ⋅ of_idx rs (IT (gReifiers_ops rs) _) sR_idx (sR_state heap))%stdpp as ->; last first.
+    { rewrite -own_op. done. }
+    unfold sR_idx. simpl.
+    intro j.
+    rewrite discrete_fun_lookup_op.
+    inv_fin j.
+    { unfold of_state, of_idx. simpl.
+      erewrite (eq_pi _ _ _ (@eq_refl _ 0%fin)). done. }
+    intros j. inv_fin j.
+    { unfold of_state, of_idx. simpl.
+      erewrite (eq_pi _ _ _ (@eq_refl _ 1%fin)). done. }
+    intros i. inversion i.
+  }
+  iApply fupd_wp.
+  iMod (inv_alloc (nroot.@"storeE") _ (∃ σ, £ 1 ∗ has_substate σ ∗ own (heapG_name rs) (●V σ))%I with "[-Hcr Hcont]") as "#Hinv".
+  { iNext. iExists _. iFrame. }
+  simpl.
+  iPoseProof (@Hlog _ _ _ with "Hcr") as "#Hlog".
+  iSpecialize ("Hlog" $! ı_scope with "[]").
+  { iIntros ([]). }
+  iSpecialize ("Hlog" $! HOM_id with "Hinv []").
+  { iApply compat_HOM_id. }
+  simpl in st.
+  iSpecialize ("Hlog" with "[$Hcont]").
+  iModIntro.
+  iApply (wp_wand with "Hlog").
+  eauto with iFrame.
+Qed.
+
+Section faulty_glue.
+  Context {sz : nat}.
+  Variable rs : gReifiers CtxDep sz.
+  Context `{!subReifier reify_delim rs}.
+  Context `{!subReifier (sReifier_NotCtxDep_min reify_store CtxDep) rs}.
+  Notation F := (gReifiers_ops rs).
+  Context {R} `{!Cofe R}.
+  Context `{!SubOfe natO R}.
+  Context `{!SubOfe unitO R}.
+  Context `{!SubOfe locO R}.
+  Notation IT := (IT F R).
+  Notation ITV := (ITV F R).
+
+  Context `{!invGS Σ, !stateG rs R Σ, !heapG rs R Σ}.
+  Notation iProp := (iProp Σ).
+
+  Program Fixpoint faulty_interp_expr {S} (e : expr S) : interp_scope S -n> IT :=
+    match e with
+    | Var x => interp_var x
+    | App n m => interp_app rs (faulty_interp_expr n) (faulty_interp_expr m)
+    | LamV e => interp_lam rs (faulty_interp_expr e)
+    | NatOp op n m => interp_natop rs op (faulty_interp_expr n) (faulty_interp_expr m)
+    | Alloc e => interp_alloc rs (faulty_interp_expr e)
+    | Assign n m => interp_assign rs (faulty_interp_expr n) (faulty_interp_expr m)
+    | Deref e => interp_deref rs (faulty_interp_expr e)
+    | LocV l => interp_loc rs l
+    | UnitV => interp_unit rs
+    | LitV n => interp_nat rs n
+    | Embed e => constO $ (embed_lang.interp_closed  _ e)
+    end.
+
+  Definition escape : embed_lang.expr ∅ :=
+    (shift/cc (# 42))%syn.
+
+  Definition buggy : expr ∅
+    := App (LamV UnitV) (Alloc (Embed escape)).
+
+  Lemma typ_buggy : typed_glued □ buggy tUnit.
+  Proof.
+    repeat econstructor.
+    Unshelve.
+    apply ℕ.
+  Qed.
+
+  Lemma faulty_spec_buggy :
+    ⊢ heap_ctx rs
+      -∗ has_substate ([] : delim.stateF ♯ IT)
+      -∗ WP@{rs} 𝒫 (faulty_interp_expr buggy ı_scope) @ notStuck
+           {{ βv, βv ≡ RetV 42
+                  ∗ has_substate ([] : delim.stateF ♯ IT)}}.
+  Proof.
+    Opaque escape.
+    iIntros "T H".
+    cbn.
+    Transparent LET.
+    unfold LET.
+    simpl.
+    do 5 example.shift_hom.
+    iApply (wp_shift with "H").
+    { rewrite laterO_map_Next. done. }
+    iIntros "!>_ H".
+    simpl.
+    iApply (wp_pop_end with "H").
+    iIntros "!>_ H".
+    simpl.
+    iApply wp_val.
+    iModIntro.
+    by iSplit.
+  Qed.
+
+  Lemma correct_spec_buggy :
+    ⊢ heap_ctx rs
+      -∗ has_substate ([] : delim.stateF ♯ IT)
+      -∗ WP@{rs} 𝒫 (interp_expr rs buggy ı_scope) @ notStuck
+           {{ βv, βv ≡ RetV ()
+                  ∗ has_substate ([] : delim.stateF ♯ IT)}}.
+  Proof.
+    Opaque escape.
+    iIntros "T H".
+    cbn.
+    Transparent LET.
+    unfold LET.
+    simpl.
+    do 5 example.shift_hom.
+    iApply (wp_reset with "H").
+    iIntros "!>_ H".
+    simpl.
+    iApply (wp_shift with "H").
+    { rewrite laterO_map_Next. done. }
+    iIntros "!>_ H".
+    simpl.
+    iApply (wp_pop_cons with "H").
+    iIntros "!>_ H".
+    simpl.
+    rewrite get_val_ITV.
+    simpl.
+    rewrite hom_vis.
+    match goal with
+    | |- context G [Vis _ _ ?a] =>
+        set (k := a);
+        eassert (k ≡ NextO ◎ (_ ◎ (Ret ◎ (subEff_outs ^-1))))%stdpp as HEQ
+    end.
+    {
+      intro; simpl.
+      rewrite later_map_Next.
+      f_equiv.
+      reflexivity.
+    }
+    rewrite HEQ.
+    match goal with
+    | HEQ : (_ ≡ NextO ◎ ?a)%stdpp |- _ =>
+        set (k' := a)
+    end.
+    match goal with
+    | |- context G [wp _ ?a] =>
+        assert (a ≡ (ALLOC (Ret 42) (𝒫 ◎ k' ◎ subEff_outs)))%stdpp as ->
+    end.
+    {
+      Transparent ALLOC.
+      unfold ALLOC.
+      rewrite hom_vis.
+      simpl.
+      f_equiv; simpl.
+      intro; simpl.
+      rewrite later_map_Next.
+      do 4 (rewrite get_val_ITV; simpl).
+      do 2 (rewrite APP'_Fun_l; simpl).
+      reflexivity.
+    }
+    Opaque ALLOC.
+    simpl.
+    clear HEQ k.
+    iApply (wp_alloc with "T"); first solve_proper.
+    iIntros "!> !> %l Hl".
+    simpl.
+    rewrite get_val_ret.
+    simpl.
+    rewrite get_val_fun.
+    simpl.
+    rewrite APP'_Fun_l.
+    simpl.
+    rewrite <-Tick_eq.
+    rewrite hom_tick.
+    iApply wp_tick.
+    iNext.
+    iApply (wp_pop_end with "H").
+    iIntros "!> _ H".
+    iApply wp_val.
+    iModIntro.
+    by iSplit.
+  Qed.
+
+End faulty_glue.
